Mathbin/Computability/Reduce.lean
@@ -310,8 +310,8 @@ theorem disjoin_manyOneReducible {α β γ} [Primcodable α] [Primcodable β] [P
     {p : α → Prop} {q : β → Prop} {r : γ → Prop} : p ≤₀ r → q ≤₀ r → p ⊕' q ≤₀ r
   | ⟨f, c₁, h₁⟩, ⟨g, c₂, h₂⟩ =>
     ⟨Sum.elim f g,
-      Computable.id.sum_cases (c₁.comp Computable.snd).to₂ (c₂.comp Computable.snd).to₂, fun x => by
-      cases x <;> [apply h₁, apply h₂]⟩
+      Computable.id.sum_casesOn (c₁.comp Computable.snd).to₂ (c₂.comp Computable.snd).to₂, fun x =>
+      by cases x <;> [apply h₁, apply h₂]⟩
 #align disjoin_many_one_reducible disjoin_manyOneReducible
 
 theorem disjoin_le {α β γ} [Primcodable α] [Primcodable β] [Primcodable γ] {p : α → Prop}
